src/ADTRefinement/FixedPoint.v
@@ -1,0 +1,964 @@
+Require Import Fiat.ADT Fiat.ADTNotation.
+Require Export Fiat.Computation.FixComp.
+
+Import LeastFixedPointFun.
+
+Instance refineFun_Reflexive fDom fCod : Reflexive (@refineFun fDom fCod).
+Proof.
+  intro x.
+  induction fDom; simpl; intros.
+  reflexivity.
+  simpl in x.
+  apply IHfDom.
+Qed.
+
+Add Parametric Morphism fDom fCod : (@refineFun fDom fCod)
+    with signature
+    ((@refineFun fDom fCod) --> (@refineFun fDom fCod) ++> impl)
+      as refineFun_refineFun.
+Proof.
+  unfold impl; intros.
+  induction fDom; simpl in *; intros.
+  rewrite H, H1, H0.
+  reflexivity.
+  specialize (IHfDom (x t) (y t) (H t) (x0 t) (y0 t)).
+  firstorder.
+Qed.
+
+Add Parametric Morphism fDom fCod : (@refineFun fDom fCod)
+    with signature
+    ((@refineFun fDom fCod) ==> Basics.flip (@refineFun fDom fCod)
+                            ==> Basics.flip impl)
+      as refineFun_refineFun_flip.
+Proof.
+  unfold impl; intros.
+  induction fDom; simpl in *; intros.
+  rewrite H, H1; assumption.
+  specialize (IHfDom (x t) (y t) (H t) (x0 t) (y0 t)).
+  firstorder.
+Qed.
+
+Instance refineFun_Transitive fDom fCod : Transitive (@refineFun fDom fCod).
+Proof.
+  intros x y z H1 H2.
+  rewrite H1.
+  exact H2.
+Qed.
+
+Program Instance refineFun_PreOrder fDom fCod : PreOrder (@refineFun fDom fCod).
+
+Definition refineFunEquiv
+           {fDom : list Type}
+           {fCod : Type}
+           (old new : funType fDom fCod) :=
+  refineFun old new /\ refineFun new old.
+
+Add Parametric Morphism fDom fCod
+  : (@refineFun fDom fCod)
+    with signature
+    (@refineFunEquiv fDom fCod) --> (@refineFunEquiv fDom fCod) ++> impl
+      as refineFun_refineFunEquiv.
+Proof.
+  unfold impl, refineFunEquiv; intros.
+  intuition.
+  rewrite H2, H1.
+  assumption.
+Qed.
+
+Add Parametric Morphism fDom fCod
+  : (@refineFun fDom fCod)
+    with signature
+    (@refineFunEquiv fDom fCod --> @refineFunEquiv fDom fCod
+                     --> Basics.flip impl)
+      as refineFun_refineFunEquiv'.
+Proof.
+  unfold impl, refineFunEquiv; intros.
+  intuition.
+  rewrite H3, H1.
+  assumption.
+Qed.
+
+Program Instance refineFunEquiv_Equivalence fDom fCod :
+  Equivalence (@refineFunEquiv fDom fCod).
+Obligation 1.
+unfold refineFunEquiv.
+intro x.
+split; reflexivity.
+Defined.
+Obligation 2.
+unfold refineFunEquiv.
+intros x y H.
+intuition.
+Qed.
+Obligation 3.
+unfold refineFunEquiv.
+intros x y z H1 H2.
+intuition.
+transitivity y; trivial.
+transitivity y; trivial.
+Qed.
+
+(*
+Corollary FixedPointP_is_refineFunEquiv
+          {fDom : list Type}
+          {fCod : Type}
+          (fDef : funType fDom fCod -> funType fDom fCod)
+          (fSet : funType fDom fCod) :
+  FixedPointP fDef fSet = refineFunEquiv (fDef fSet) fSet.
+Proof. reflexivity. Qed.
+ *)
+
+Instance refineFun_refineFunEquiv_subrelation fDom fCod :
+  subrelation (@refineFunEquiv fDom fCod) (@refineFun fDom fCod).
+Proof. intros ? ? [? ?]; assumption. Qed.
+
+(*
+Add Parametric Morphism fDom fCod : (@FixedPointP fDom fCod)
+  with signature
+    ((@refineFunEquiv fDom fCod) ==> (@refineFunEquiv fDom fCod))
+       ==> (@refineFunEquiv fDom fCod) ==> impl
+    as refineFun_FixedPointP.
+Proof.
+  unfold respectful, FixedPointP, refineFunEquiv, impl; simpl; intros.
+  specialize (H _ _ H0).
+  intuition.
+  - rewrite H3, H0; assumption.
+  - rewrite H2 in H5.
+    rewrite H5 in H4.
+    assumption.
+Qed.
+ *)
+
+Lemma length_wf' : forall A len l,
+    length l < len -> Acc (fun l1 l2 : list A => length l1 < length l2) l.
+Proof.
+  induction len; simpl; intros;
+    constructor; intros.
+  contradiction (NPeano.Nat.nlt_0_r _ H).
+  apply IHlen.
+  Require Import Omega.
+  omega.
+Qed.
+
+Lemma length_wf : forall A,
+    well_founded (fun l1 l2 : list A => length l1 < length l2).
+Proof.
+  red; intros; eapply length_wf'; eauto.
+Qed.
+
+Definition funType_to_methodType
+           {rep : Type} {dom : list Type} {cod : Type} :
+  funType (rep :: dom) (rep * cod) -> methodType rep dom (Some cod).
+Proof.
+  simpl; intro f.
+  intro r'.
+  specialize (f r'); clear r'.
+  induction dom; simpl in *.
+  exact f.
+  intro r'.
+  exact (IHdom (f r')).
+Defined.
+
+Definition methodType_to_funType
+           {rep : Type} {dom : list Type} {cod : Type} :
+  methodType rep dom (Some cod) -> funType (rep :: dom) (rep * cod).
+Proof.
+  simpl; intro f.
+  intro r'.
+  specialize (f r'); clear r'.
+  induction dom; simpl in *.
+  exact f.
+  intro r'.
+  exact (IHdom (f r')).
+Defined.
+
+Lemma methodType_to_funType_id
+      {rep : Type} {dom : list Type} {cod : Type}
+      (f : funType (rep :: dom) (rep * cod)) :
+  methodType_to_funType (funType_to_methodType f) = f.
+Proof.
+  unfold methodType_to_funType, funType_to_methodType.
+  extensionality r.
+  induction dom; simpl in f;
+    extensionality x; simpl.
+  reflexivity.
+  exact (IHdom (fun r => f r x)).
+Qed.
+
+Import EqNotations.
+
+Require Import Fiat.Common.Frame.
+
+Inductive hetero {A : Type} {B : A -> Type} : list A -> Type :=
+| hnil : hetero []
+| hcons x xs : hetero xs -> B x -> hetero (x :: xs).
+
+Ltac under_fDom :=
+  match goal with
+  | [ fDom : list Type |- _ ] =>
+    induction fDom; simpl in *;
+    [| intros;
+       repeat
+         match goal with
+         | [ f : ?OLDREP -> ?A -> funType ?FDOM ?FCOD |- _ ] =>
+           match goal with
+             [ IHfDom : (OLDREP -> funType FDOM FCOD) -> _,
+                        x : A |- _ ] =>
+             specialize (IHfDom (fun r => f r x));
+             try exact IHfDom;
+             try clear f
+           end
+         | [ f : ?OLDREP -> ?A -> methodType' ?OLDREP ?FDOM ?FCOD |- _ ] =>
+           match goal with
+             [ IHfDom : (OLDREP -> methodType' OLDREP FDOM FCOD) -> _,
+                        x : A |- _ ] =>
+             specialize (IHfDom (fun r => f r x));
+             try exact IHfDom;
+             try clear f
+           end
+         | [ f : ?A -> funType ?FDOM ?FCOD |- _ ] =>
+           match goal with
+             [ IHfDom : funType FDOM FCOD -> _,
+                        x : A |- _ ] =>
+             specialize (IHfDom (f x));
+             try exact IHfDom;
+             try clear f
+           end
+         end ]
+  end.
+
+Definition funApply {fDom fCod} :
+  funType fDom fCod -> hetero (B:=id) fDom -> Comp fCod.
+Proof.
+  intros.
+  induction fDom; simpl in *.
+  exact X.
+  inversion X0.
+  exact (IHfDom (X X2) X1).
+Defined.
+
+Definition dom_old_to_new {newRep oldRep fDom fCod}
+           (AbsR : oldRep -> newRep -> Prop) :
+  funType (oldRep :: fDom) fCod -> funType (newRep :: fDom) fCod.
+Proof.
+  simpl; intros f r_n.
+  induction fDom; simpl in *.
+  exact ({ v | exists (r_o : oldRep),
+               AbsR r_o r_n -> computes_to (f r_o) v}).
+  exact (fun x => IHfDom (fun r => f r x)).
+Defined.
+
+Definition cod_old_to_new {newRep oldRep fDom fCod}
+           (AbsR : oldRep -> newRep -> Prop) :
+  funType fDom (oldRep * fCod) -> funType fDom (newRep * fCod).
+Proof.
+  simpl; intros f.
+  induction fDom; simpl in *.
+  exact (p <- f;
+         n <- { n : newRep | AbsR (fst p) n };
+         ret (n, snd p)).
+  intro x.
+  exact (IHfDom (f x)).
+Defined.
+
+Definition dom_new_to_old {newRep oldRep fDom fCod}
+           (AbsR : oldRep -> newRep -> Prop) :
+  funType (newRep :: fDom) fCod -> funType (oldRep :: fDom) fCod.
+Proof.
+  simpl; intros f o.
+  induction fDom; simpl in *.
+  exact (n <- { n : newRep | AbsR o n };
+         f n).
+  intro x.
+  exact (IHfDom (fun r => f r x)).
+Defined.
+
+Definition cod_new_to_old {newRep oldRep fDom fCod}
+           (AbsR : oldRep -> newRep -> Prop) :
+  funType fDom (newRep * fCod) -> funType fDom (oldRep * fCod).
+Proof.
+  simpl; intros f.
+  induction fDom; simpl in *.
+  exact (p <- f;
+         o <- { o : oldRep | AbsR o (fst p) };
+         ret (o, snd p)).
+  intro x.
+  exact (IHfDom (f x)).
+Defined.
+
+Definition domcod_old_to_new {newRep oldRep fDom fCod}
+           (AbsR : oldRep -> newRep -> Prop) :
+  funType (oldRep :: fDom) (oldRep * fCod) ->
+  funType (newRep :: fDom) (newRep * fCod) :=
+  fun k nr => cod_old_to_new AbsR (dom_old_to_new AbsR k nr).
+
+Definition domcod_new_to_old {newRep oldRep fDom fCod}
+           (AbsR : oldRep -> newRep -> Prop) :
+  funType (newRep :: fDom) (newRep * fCod) ->
+  funType (oldRep :: fDom) (oldRep * fCod) :=
+  fun k nr => cod_new_to_old AbsR (dom_new_to_old AbsR k nr).
+
+Definition funType_join {fDom fCod} :
+  Comp (funType fDom fCod) -> funType fDom fCod.
+Proof.
+  intros.
+  induction fDom.
+  exact (v <- X; v).
+  intro x.
+  exact (IHfDom (f <- X; ret (f x))).
+Defined.
+
+Definition refineFun_invert
+           {newRep oldRep fDom fCod}
+           (AbsR : oldRep -> newRep -> Prop)
+           (f : funType (oldRep :: fDom) (oldRep * fCod))
+           (f' : funType (newRep :: fDom) (newRep * fCod)) :
+  (forall (args : hetero fDom),
+      pointwise_relation _ refine
+                         (fun or =>
+                            p <- funApply (f or) args;
+                              n <- { n : newRep | AbsR (fst p) n };
+                              ret (n, snd p))
+                         (fun or =>
+                            n <- { n : newRep | AbsR or n };
+                              funApply (f' n) args))
+  -> refineFun (cod_old_to_new AbsR f)
+               (dom_new_to_old AbsR f').
+Proof.
+  intros H.
+  under_fDom.
+  exact (H hnil).
+  apply IHfDom; intros.
+  exact (H (hcons (B:=id) _ args t0)).
+Defined.
+
+Require Import
+        Fiat.ADTRefinement
+        Fiat.ADTRefinement.BuildADTRefinements.
+
+Lemma refineFunMethod :
+  forall oldRep newRep (AbsR : oldRep -> newRep -> Prop) fDom fCod
+         (f : methodType oldRep fDom (Some fCod))
+         (f' : methodType newRep fDom (Some fCod)),
+    refineFun (cod_old_to_new AbsR (methodType_to_funType f))
+              (dom_new_to_old AbsR (methodType_to_funType f'))
+    -> refineMethod AbsR f f'.
+Proof.
+  unfold dom_new_to_old, refineMethod,
+  methodType, methodType_to_funType; simpl in *; intros.
+  specialize (H r_o).
+  under_fDom.
+  rewrite H.
+  refine pick val r_n.
+  simplify with monad laws; simpl.
+  reflexivity.
+  exact H0.
+  apply IHfDom.
+  rewrite H.
+  f_equiv.
+Defined.
+
+Fixpoint refineFun_AbsR'
+         {oldRep newRep}
+         (fDom : list Type)
+         (fCod : Type)
+         (AbsR : oldRep -> newRep -> Prop)
+         (fDef : funType fDom (oldRep * fCod))
+         (fDef' : funType fDom (newRep * fCod))
+         {struct fDom} : Prop :=
+  match fDom as fDom'
+        return funType fDom' (oldRep * fCod)
+               -> funType fDom' (newRep * fCod) -> Prop
+  with
+  | List.nil =>
+    fun fDef fDef' => refine (cod_old_to_new AbsR fDef) fDef'
+  | List.cons T fDom' =>
+    fun fDef fDef' =>
+      forall (t : T), refineFun_AbsR' fDom' fCod AbsR (fDef t) (fDef' t)
+  end fDef fDef'.
+
+Definition refineFun_AbsR
+           {oldRep newRep}
+           (AbsR : oldRep -> newRep -> Prop)
+           {fDom : list Type}
+           {fCod : Type}
+           (fDef : funType (oldRep :: fDom) (oldRep * fCod))
+           (fDef' : funType (newRep :: fDom) (newRep * fCod)) : Prop :=
+  forall r_o r_n, AbsR r_o r_n
+                  -> refineFun_AbsR' fDom fCod AbsR (fDef r_o) (fDef' r_n).
+
+Lemma refineFun_AbsR_trans
+      {oldRep newRep}
+      (AbsR : oldRep -> newRep -> Prop)
+      {fDom : list Type}
+      {fCod : Type}
+  : forall (fDef fDef'' : funType (oldRep :: fDom) (oldRep * fCod))
+           (fDef' : funType (newRep :: fDom) (newRep * fCod)),
+    refineFun fDef fDef''
+    -> refineFun_AbsR AbsR fDef'' fDef'
+    -> refineFun_AbsR AbsR fDef fDef'.
+Proof.
+  intros.
+  unfold refineFun_AbsR in *.
+  induction fDom; simpl in *; intros.
+  rewrite H.
+  exact (H0 _ _ H1).
+  apply (IHfDom (fun r => fDef r t)
+                (fun r => fDef'' r t)
+                (fun r => fDef' r t)).
+  - intros.
+    exact (H _ _).
+  - intros.
+    exact (H0 _ _ H2 _).
+  - exact H1.
+Qed.
+
+Lemma refineFun_AbsR'_trans
+      {oldRep newRep}
+      (AbsR : oldRep -> newRep -> Prop)
+      {fDom : list Type}
+      {fCod : Type}
+  : forall (fDef fDef'' : funType fDom (oldRep * fCod))
+           (fDef' : funType fDom (newRep * fCod)),
+    refineFun fDef fDef''
+    -> refineFun_AbsR' _ _ AbsR fDef'' fDef'
+    -> refineFun_AbsR' _ _ AbsR fDef fDef'.
+Proof.
+  intros.
+  induction fDom; simpl in *; intros.
+  rewrite H; eauto.
+  eauto.
+Qed.
+
+Lemma refineFun_AbsR_trans'
+      {oldRep newRep}
+      (AbsR : oldRep -> newRep -> Prop)
+      {fDom : list Type}
+      {fCod : Type}
+  : forall (fDef : funType (oldRep :: fDom) (oldRep * fCod))
+           (fDef' fDef'' : funType (newRep :: fDom) (newRep * fCod)),
+    refineFun fDef'' fDef'
+    -> refineFun_AbsR AbsR fDef fDef''
+    -> refineFun_AbsR AbsR fDef fDef'.
+Proof.
+  intros.
+  unfold refineFun_AbsR in *.
+  induction fDom; simpl in *; intros.
+  rewrite (H0 _ _ H1).
+  exact (H _).
+  apply (IHfDom (fun r => fDef r t)
+                (fun r => fDef' r t)
+                (fun r => fDef'' r t)).
+  - intros.
+    exact (H _ _).
+  - intros.
+    exact (H0 _ _ H2 _).
+  - exact H1.
+Qed.
+
+(*Lemma refineFun_To_refineFunAbsR'
+      {oldRep newRep}
+      (AbsR : oldRep -> newRep -> Prop)
+      {fDom : list Type}
+      {fCod : Type}
+  : forall (fDef  : funType (oldRep :: fDom) (oldRep * fCod))
+           (fDef' : funType (newRep :: fDom) (newRep * fCod)),
+    refineFun fDef (dom_new_to_old AbsR fDef')
+    <-> refineFun (cod_old_to_new AbsR fDef) fDef'.
+    forall r_o r_n, AbsR r_o r_n
+      -> (forall r_o r_n, refineFun_AbsR' fDom fCod AbsR (fDef r_o) (fDef' r_n))
+      -> refineFun  (dom_new_to_old AbsR fDef').
+Proof.
+  intros.
+  unfold refineFun_AbsR', cod_old_to_new, dom_new_to_old in *.
+  under_fDom.
+    intros.
+    rewrite (H0 t r_n).
+    unfold refine; intros.
+    apply Bind_inv in H1.
+    do 2 destruct H1.
+    apply Pick_inv in H1.
+    admit.
+  Fail apply (IHfDom (fun r => H r t)).
+Admitted.
+ *)
+
+Lemma refineFun_To_refineFunAbsR'
+      {oldRep newRep}
+      (AbsR : oldRep -> newRep -> Prop)
+      {fDom : list Type}
+      {fCod : Type}
+  : forall (fDef  : funType (fDom) (oldRep * fCod))
+           (fDef' : funType (fDom) (newRep * fCod)),
+    refineFun (cod_old_to_new AbsR fDef) fDef'
+    <-> refineFun_AbsR' _ _ AbsR fDef fDef'.
+Proof.
+  induction fDom; simpl; eauto.
+  - split; eauto.
+  - split; intros; eapply IHfDom; eauto.
+Qed.
+
+(*Lemma refineFun_To_refineFunAbsR
+      {oldRep newRep}
+      (AbsR : oldRep -> newRep -> Prop)
+      {fDom : list Type}
+      {fCod : Type}
+  : forall (fDef  : funType (oldRep :: fDom) (oldRep * fCod))
+           (fDef' : funType (newRep :: fDom) (newRep * fCod)),
+    refineFun (domcod_old_to_new AbsR fDef) fDef'
+    -> refineFun_AbsR AbsR fDef fDef'.
+Proof.
+  simpl.
+  setoid_rewrite refineFun_To_refineFunAbsR'.
+  intros.
+  unfold refineFun_AbsR; induction fDom; simpl in *; eauto.
+  - intros; rewrite <- H; unfold refine; intros.
+    computes_to_inv; subst; eauto.
+    destruct_ex.
+  - intros;
+      eapply (IHfDom (fun r => fDef r t) (fun r => fDef' r t)); eauto.
+Qed. *)
+
+Lemma refineFunAbsR_To_refineFun
+      {oldRep newRep}
+      (AbsR : oldRep -> newRep -> Prop)
+      {fDom : list Type}
+      {fCod : Type}
+  : forall (fDef : funType (oldRep :: fDom) (oldRep * fCod))
+           (fDef' : funType (newRep :: fDom) (newRep * fCod)),
+    refineFun (cod_old_to_new AbsR fDef) (dom_new_to_old AbsR fDef')
+    <-> refineFun_AbsR AbsR fDef fDef'.
+Proof.
+  intros.
+  unfold refineFun_AbsR, cod_old_to_new, dom_new_to_old.
+  under_fDom.
+  { split; intros.
+    - setoid_rewrite H.
+      refine pick val r_n.
+      simplify with monad laws.
+      reflexivity.
+      exact H0.
+    - unfold refine; intros; computes_to_inv.
+      eapply H in H0'; eauto.
+  }
+  split; intros.
+  eapply (IHfDom (fun r => fDef r t) (fun r => fDef' r t)); eauto.
+  eapply (IHfDom (fun r => fDef r t0) (fun r => fDef' r t0)); eauto.
+Qed.
+
+Lemma cod_old_to_new_monotone
+      {oldRep newRep}
+      (AbsR : oldRep -> newRep -> Prop)
+      {fDom : list Type}
+      {fCod : Type}
+  : forall (fDef fDef' : funType fDom (oldRep * fCod)),
+    refineFun fDef fDef'
+    -> refineFun (cod_old_to_new AbsR fDef) (cod_old_to_new AbsR fDef').
+Proof.
+  induction fDom; simpl; intros.
+  -setoid_rewrite H; reflexivity.
+  - simpl; eauto.
+Qed.
+
+Lemma domcod_old_to_new_monotone
+      {oldRep newRep}
+      (AbsR : oldRep -> newRep -> Prop)
+      {fDom : list Type}
+      {fCod : Type}
+  : forall (fDef fDef'  : funType (oldRep :: fDom) (oldRep * fCod)),
+    refineFun fDef fDef'
+    -> refineFun (domcod_old_to_new AbsR fDef) (domcod_old_to_new AbsR fDef').
+Proof.
+  induction fDom; simpl; intros.
+  - unfold domcod_old_to_new; simpl.
+    setoid_rewrite H; reflexivity.
+  - unfold domcod_old_to_new in *.
+    simpl; eapply (IHfDom (fun r => fDef r t0) (fun r => fDef' r t0)); eauto.
+    simpl; eauto.
+Qed.
+
+(*Lemma domcod_old_to_new_resp_sup'
+      {oldRep newRep}
+      (AbsR : oldRep -> newRep -> Prop)
+      {fDom : list Type}
+      {fCod : Type}
+  : forall P,
+    refineFun (@domcod_old_to_new _ _ fDom fCod AbsR (cl_sup P))
+              (cl_sup (fun f (* new Point *) =>
+                         exists f',
+                           P f'
+                           /\ f = @domcod_old_to_new _ _ fDom fCod AbsR f')). *)
+
+Lemma domcod_old_to_new_resp_inf_1'
+      {oldRep newRep}
+      (AbsR : oldRep -> newRep -> Prop)
+      {fDom : list Type}
+      {fCod : Type}
+  : forall P,
+    refineFun (@domcod_old_to_new _ _ fDom fCod AbsR (cl_inf P))
+              (cl_inf (fun f (* new Point *) =>
+                         exists f',
+                           P f'
+                           /\ refineFun (@domcod_old_to_new _ _ fDom fCod AbsR f') f)).
+Proof.
+  intros; eapply (glb_refineFun_inf _ (fun f (* new Point *) =>
+                         exists f',
+                           P f'
+                           /\ refineFun (@domcod_old_to_new _ _ fDom fCod AbsR f') f)).
+  simpl; intros; destruct_ex; intuition subst.
+  rewrite <- H1.
+  eapply domcod_old_to_new_monotone.
+  eapply (glb_refineFun_inf _ P); eauto.
+Qed.
+
+Lemma domcod_old_to_new_resp_inf_2'
+      {oldRep newRep}
+      (AbsR : oldRep -> newRep -> Prop)
+      {fDom : list Type}
+      {fCod : Type}
+  : forall P,
+    P (refineFun_inf P)
+    -> refineFun (cl_inf (fun f (* new Point *) =>
+                         exists f',
+                           P f'
+                           /\ refineFun (@domcod_old_to_new _ _ fDom fCod AbsR f') f))
+              (@domcod_old_to_new _ _ fDom fCod AbsR (cl_inf P))
+.
+Proof.
+  intros; eapply (glb_refineFun_inf _ (fun f (* new Point *) =>
+                         exists f',
+                           P f'
+                           /\ refineFun (@domcod_old_to_new _ _ fDom fCod AbsR f') f)).
+  simpl; intros; destruct_ex; intuition subst.
+  eexists (refineFun_inf P); split; intros; eauto.
+  reflexivity.
+Qed.
+
+Definition domcod_new_to_old'
+           {newRep oldRep fDom fCod}
+           (AbsR : oldRep -> newRep -> Prop)
+           (fDef' : funType (newRep :: fDom) (newRep * fCod))
+  : funType (oldRep :: fDom) (oldRep * fCod) :=
+  cl_sup (fun a : funType (oldRep :: fDom) (oldRep * fCod) =>
+            refineFun (domcod_old_to_new AbsR a) fDef').
+
+(* Lemma domcod_new_to_old_resp_inf_2' *)
+(*       {oldRep newRep} *)
+(*       (AbsR : oldRep -> newRep -> Prop) *)
+(*       {fDom : list Type} *)
+(*       {fCod : Type} *)
+(*   : forall P, *)
+(*     P (refineFun_inf P) *)
+(*     -> refineFun (cl_inf (fun f (* new Point *) => *)
+(*                          exists f', *)
+(*                            P f' *)
+(*                            /\ refineFun (@domcod_new_to_old' _ _ fDom fCod AbsR f') f)) *)
+(*               (@domcod_new_to_old' _ _ fDom fCod AbsR (cl_inf P)) *)
+(* . *)
+(* Proof. *)
+(*   intros; eapply (glb_refineFun_inf _ (fun f (* new Point *) => *)
+(*                          exists f', *)
+(*                            P f' *)
+(*                            /\ refineFun (@domcod_old_to_new _ _ fDom fCod AbsR f') f)). *)
+(*   simpl; intros; destruct_ex; intuition subst. *)
+(*   eexists (refineFun_inf P); split; intros; eauto. *)
+(*   reflexivity. *)
+(* Qed. *)
+
+Lemma domcod_old_to_new_resp_sup_1'
+      {oldRep newRep}
+      (AbsR : oldRep -> newRep -> Prop)
+      {fDom : list Type}
+      {fCod : Type}
+  : forall P,
+    refineFun (cl_sup (fun f (* new Point *) =>
+                         exists f',
+                           P f'
+                           /\ refineFun f (@domcod_old_to_new _ _ fDom fCod AbsR f')))
+              (@domcod_old_to_new _ _ fDom fCod AbsR (cl_sup P))
+.
+Proof.
+  intros; eapply (lub_refineFun_sup _ (fun f (* new Point *) =>
+                         exists f',
+                           P f'
+                           /\ refineFun f (@domcod_old_to_new _ _ fDom fCod AbsR f'))).
+  simpl; intros; destruct_ex; intuition subst.
+  rewrite H1.
+  eapply domcod_old_to_new_monotone.
+  eapply (lub_refineFun_sup _ P); eauto.
+Qed.
+
+Lemma domcod_old_to_new_resp_sup_2'
+      {oldRep newRep}
+      (AbsR : oldRep -> newRep -> Prop)
+      {fDom : list Type}
+      {fCod : Type}
+  : forall P,
+    P (refineFun_sup P)
+    -> refineFun
+         (@domcod_old_to_new _ _ fDom fCod AbsR (cl_sup P))
+         (cl_sup (fun f (* new Point *) =>
+                    exists f',
+                      P f'
+                      /\ refineFun f (@domcod_old_to_new _ _ fDom fCod AbsR f'))).
+Proof.
+  intros.
+  eapply (lub_refineFun_sup _ (fun f (* new Point *) =>
+                                 exists f',
+                                   P f'
+                           /\ refineFun f (@domcod_old_to_new _ _ fDom fCod AbsR f'))).
+  eexists (refineFun_sup P); intuition.
+Qed.
+
+(*Lemma domcod_old_to_new_resp_sup_2'
+      {oldRep newRep}
+      (AbsR : oldRep -> newRep -> Prop)
+      {fDom : list Type}
+      {fCod : Type}
+  : forall P,
+    refineFun (cl_sup (fun f (* new Point *) =>
+                         exists f',
+                           P f'
+                           /\ refineFunEquiv f (@domcod_old_to_new _ _ fDom fCod AbsR f')))
+              (@domcod_old_to_new _ _ fDom fCod AbsR (cl_sup P)).
+Proof.
+  intros; eapply (glb_refineFun_sup _ (fun f (* new Point *) =>
+                         exists f',
+                           P f'
+                           /\ refineFunEquiv f (@domcod_old_to_new _ _ fDom fCod AbsR f'))).
+  eexists (refineFun_sup P); intuition.
+  destruct (glb_refineFun_sup _ P).
+  simpl in *.
+  eapply H; eauto.
+Qed.
+
+
+  (fDef fDef'  : funType (oldRep :: fDom) (oldRep * fCod)),
+    refineFun fDef fDef'
+    -> refineFun (domcod_old_to_new AbsR fDef) (domcod_old_to_new AbsR fDef').
+Proof.
+  induction fDom; simpl; intros.
+  - unfold domcod_old_to_new; simpl.
+    setoid_rewrite H; reflexivity.
+  - unfold domcod_old_to_new in *.
+    simpl; eapply (IHfDom (fun r => fDef r t0) (fun r => fDef' r t0)); eauto.
+    simpl; eauto.
+Qed. *)
+
+(*Lemma domcod_old_to_new_roundtrip
+      {newRep oldRep fDom fCod}
+      (AbsR : oldRep -> newRep -> Prop)
+  : forall (fDef' : funType (newRep :: fDom) (newRep * fCod))
+           (t : newRep),
+    refineFun (domcod_old_to_new AbsR (domcod_new_to_old' AbsR fDef') t) (fDef' t).
+Proof.
+  induction fDom; simpl.
+  - unfold domcod_new_to_old', domcod_old_to_new; simpl.
+    unfold refine; intros.
+    destruct v.
+    computes_to_econstructor.
+    apply PickComputes with (a := (t, f)).
+    intros.
+
+    unfold refineFun_sup; simpl.
+    Local Transparent computes_to.
+
+    unfold computes_to.
+    eexists; split; eauto.
+    Focus 2.
+    apply H0.
+
+
+    unfold ref
+ *)
+
+Lemma domcod_new_to_old'_OK'
+      {newRep oldRep fDom fCod}
+      (AbsR : oldRep -> newRep -> Prop)
+  : forall (fDef : funType (oldRep :: fDom) (oldRep * fCod))
+           (fDef' : funType (newRep :: fDom) (newRep * fCod))
+           r_o r_n,
+    AbsR r_o r_n
+    -> (refineFun (fDef r_o) (domcod_new_to_old' AbsR fDef' r_o) <->
+        refineFun (domcod_old_to_new AbsR fDef r_n) (fDef' r_n)).
+Proof.
+  split; intros.
+  - simpl in *; intros.
+    unfold domcod_new_to_old' in *.
+    eapply (cod_old_to_new_monotone AbsR) in H0.
+    unfold domcod_old_to_new. (* rewrite H0.
+    rewrite domcod_old_to_new_resp_sup_2'.
+    destruct (sup_lub (fun f : funType (newRep :: fDom) (newRep * fCod) =>
+         exists f' : funType (oldRep :: fDom) (oldRep * fCod), refineFun (domcod_old_to_new AbsR f') fDef' /\ refineFun f (domcod_old_to_new AbsR f'))).
+    simpl in *; eapply H1.
+    intros.
+    destruct_ex; intuition.
+    rewrite <- H3, H4; reflexivity. *)
+    admit.
+    (*pose proof @domcod_old_to_new_resp_sup_2'.
+
+    simpl in H0; simpl in *.
+    intros; rewrite (H0 _ _ AbsR _ _ (fun a : funType (oldRep :: fDom) (oldRep * fCod) => refineFun (domcod_old_to_new AbsR a) fDef')).
+    admit. *)
+  - simpl in *.
+    unfold domcod_new_to_old'; intros.
+    destruct (sup_lub (fun a : funType fDom (oldRep * fCod) => refineFun (cod_old_to_new AbsR a) (fDef' r_n))).
+    admit.
+Qed.
+
+Lemma domcod_new_to_old'_OK
+      {newRep oldRep fDom fCod}
+      (AbsR : oldRep -> newRep -> Prop)
+  : forall (fDef : funType (oldRep :: fDom) (oldRep * fCod))
+           (fDef' : funType (newRep :: fDom) (newRep * fCod)),
+    refineFun fDef (domcod_new_to_old' AbsR fDef') <->
+    refineFun (domcod_old_to_new AbsR fDef) fDef'.
+Proof.
+Admitted.
+(*  split; intros.
+  - simpl in *; intros.
+    unfold domcod_new_to_old' in *.
+    eapply (domcod_old_to_new_monotone AbsR) in H0.
+    rewrite H.
+    rewrite domcod_old_to_new_resp_sup_2'.
+    destruct (sup_lub (fun f : funType (newRep :: fDom) (newRep * fCod) =>
+         exists f' : funType (oldRep :: fDom) (oldRep * fCod), refineFun (domcod_old_to_new AbsR f') fDef' /\ refineFun f (domcod_old_to_new AbsR f'))).
+    simpl in *; eapply H1.
+    intros.
+    destruct_ex; intuition.
+    rewrite <- H3, H4; reflexivity.
+    admit.
+    (*pose proof @domcod_old_to_new_resp_sup_2'.
+
+    simpl in H0; simpl in *.
+    intros; rewrite (H0 _ _ AbsR _ _ (fun a : funType (oldRep :: fDom) (oldRep * fCod) => refineFun (domcod_old_to_new AbsR a) fDef')).
+    admit. *)
+  - simpl in *.
+    unfold domcod_new_to_old'; intros.
+    destruct (sup_lub (fun a : funType (oldRep :: fDom) (oldRep * fCod) => refineFun (domcod_old_to_new AbsR a) fDef')).
+    simpl in *.
+    rewrite H0; eauto.
+Qed. *)
+
+Lemma refineFun_AbsR_unCurry
+      {oldRep newRep}
+      (AbsR : oldRep -> newRep -> Prop)
+      {fDom : list Type}
+      {fCod : Type}
+  : forall (fDef : funType fDom (oldRep * fCod))
+           (fDef' : funType fDom (newRep * fCod)),
+    refineFun_AbsR' _ _ AbsR fDef fDef'
+    -> refineFun_AbsR' _ _ AbsR (unCurry _ fDef) (unCurry _ fDef').
+  Proof.
+    induction fDom; simpl.
+    - intros; eauto.
+    - intros.
+      eapply IHfDom; eauto.
+  Qed.
+
+Lemma refineFun_AbsR_unCurry'
+      {oldRep newRep}
+      (AbsR : oldRep -> newRep -> Prop)
+      {fDom : list Type}
+      {fCod : Type}
+  : forall (fDef : funType fDom (oldRep * fCod))
+           (fDef' : funType fDom (newRep * fCod)),
+    refineFun_AbsR' _ _ AbsR (unCurry _ fDef) (unCurry _ fDef')
+    -> refineFun_AbsR' _ _ AbsR fDef fDef'.
+  Proof.
+    induction fDom; simpl.
+    - intros; eapply (H tt).
+    - intros.
+      eapply IHfDom; eauto.
+      simpl; intros.
+      eapply (H (t, t0)).
+  Qed.
+
+  Lemma foo
+        {oldRep newRep}
+        (AbsR : oldRep -> newRep -> Prop)
+        {fDom : list Type}
+        {fCod : Type}
+        (fDef' : funType (newRep :: fDom) (newRep * fCod))
+    : forall t0 t1,
+      refineEquiv
+        (unCurry fDom (domcod_new_to_old' AbsR fDef' t0) t1)
+        (@domcod_new_to_old' _ _ [_] _ AbsR (fun r_n t1 => unCurry _ fDef' (r_n, t1)) t0 t1).
+  Admitted.
+
+  Lemma refine_LeastFixedPoint_AbsR'
+      {oldRep newRep}
+      (AbsR : oldRep -> newRep -> Prop)
+      {fDom : list Type}
+      {fCod : Type}
+      (fDef : funType (oldRep :: fDom) (oldRep * fCod)
+              -> funType (oldRep :: fDom) (oldRep * fCod))
+      (fDef' : funType (newRep :: fDom) (newRep * fCod))
+      (fDef_monotone : forall rec rec',
+          refineFun rec rec'
+          -> refineFun (fDef rec) (fDef rec'))
+      (_ : refineFun_AbsR AbsR (fDef (domcod_new_to_old' AbsR fDef')) fDef')
+  : refineFun_AbsR AbsR (refineFun_inf (prefixed_point fDef)) fDef'.
+Proof.
+  intros r_o r_n AbsR'.
+  eapply refineFun_AbsR_unCurry'.
+  generalize H; intros H'.
+  eapply refineFun_AbsR_unCurry in H; eauto; simpl in *.
+  intros.
+  rewrite <- H.
+  f_equiv.
+  eapply refineFun_unCurry.
+  pose proof (proj1 (Is_LeastFixedPoint
+                       (O := @funDefOps (oldRep :: fDom) (oldRep * fCod))
+                       _ (fDef_monotone))) as H1;
+    simpl in H1; rewrite H1; clear H1.
+  apply fDef_monotone.
+  intros.
+  eapply refineFun_unCurry'; simpl; intros.
+  rewrite foo.
+  simpl.
+  unfold domcod_new_to_old'.
+  simpl.
+  unfold refineFun_sup; simpl.
+  Local Transparent computes_to.
+  unfold refine, computes_to; intros. simpl in *.
+  eapply H0.
+  intros.
+  admit.
+Admitted.
+
+Lemma refine_LeastFixedPoint_AbsR
+      {oldRep newRep}
+      (AbsR : oldRep -> newRep -> Prop)
+      {fDom : list Type}
+      {fCod : Type}
+      (fDef : funType (oldRep :: fDom) (oldRep * fCod)
+              -> funType (oldRep :: fDom) (oldRep * fCod))
+      (fDef' : funType (newRep :: fDom) (newRep * fCod)
+               -> funType (newRep :: fDom) (newRep * fCod))
+  : respectful_hetero
+      (funType (oldRep :: fDom) (oldRep * fCod))
+      (funType (newRep :: fDom) (newRep * fCod))
+      (fun _ => funType (oldRep :: fDom) (oldRep * fCod))
+      (fun _ => funType (newRep :: fDom) (newRep * fCod))
+      (fun f f' => @refineFun_AbsR _ _ AbsR fDom fCod f f')
+      (fun rec rec' f f' =>
+         @refineFun_AbsR _ _ AbsR fDom fCod f f')
+      fDef fDef'
+    -> forall (fDef_monotone : forall rec rec',
+                  refineFun rec rec'
+                  -> refineFun (fDef rec) (fDef rec'))
+              (fDef'_monotone : forall rec rec',
+                  refineFun rec rec'
+                  -> refineFun (fDef' rec) (fDef' rec')),
+      refineFun_AbsR AbsR (LeastFixedPoint fDef)
+                     (LeastFixedPoint fDef').
+Proof.
+  unfold LeastFixedPoint, respectful_hetero; intros.
+  eapply refine_LeastFixedPoint_AbsR'; eauto.
+  eapply refineFun_AbsR_trans'.
+  rewrite <- Is_LeastFixedPoint; eauto; reflexivity.
+  eapply H.
+  simpl.
+  admit.
+Qed.
